library/init/meta/ttactic.lean
@@ -1,0 +1,280 @@
+namespace ttactic
+open tactic
+
+/-- Goals can be tagged using a list of names. -/
+def tag : Type := list name
+
+meta structure tag_info :=
+(tags_enabled : bool)
+(tags         : expr_map (list name))
+
+/-- A 'tagged tactic' -/
+@[reducible] meta def ttactic :=
+state_t tag_info tactic
+
+meta instance : monad_tactic ttactic :=
+_root_.monad_tactic.mk infer_instance infer_instance infer_instance infer_instance
+
+section
+parameters {m n : Type → Type} [monad_tactic m] [monad_state_lift tag_info n m] [monad n]
+include n
+
+/-- Enable/disable goal tagging -/
+meta def enable_tags (b : bool) : m punit :=
+modify (λ s, { tags_enabled := b, ..s })
+
+/-- Return tt iff goal tagging is enabled. -/
+meta def tags_enabled : m bool :=
+tag_info.tags_enabled <$> get
+
+/-- Tag goal `g` with tag `t`. It does nothing is goal tagging is disabled.
+    Remark: `set_goal g []` removes the tag -/
+meta def set_tag (g : expr) (t : tag) : m unit :=
+mwhen tags_enabled $
+modify (λ s, { tags := if t = [] then s.tags.erase g
+                                 else s.tags.insert g t, ..s }) >> pure ()
+
+/-- Return tag associated with `g`. Return `[]` if there is no tag. -/
+meta def get_tag (g : expr) : m tag :=
+do s ← get, pure $ (s.tags.find g).get_or_else []
+
+/- Goal tagging support -/
+meta def with_enable_tags {α : Type} (t : m α) (b := tt) : m α :=
+do old ← tags_enabled,
+   enable_tags b,
+   r ← t,
+   enable_tags old,
+   return r
+
+meta def get_main_tag : m tag :=
+main_goal >>= get_tag
+
+meta def set_main_tag (t : tag) : m unit :=
+do g ← main_goal, set_tag g t
+
+meta def propagate_tags (tac : m unit) : m unit :=
+do tag ← get_main_tag,
+   if tag = [] then tac
+   else focus1 $ do
+     tac,
+     gs ← get_goals,
+     when (bnot gs.empty) $ do
+       new_tag ← get_main_tag,
+       when new_tag.empty $ with_enable_tags (set_main_tag tag)
+
+meta def concat_tags (tac : m (list (name × expr))) : m unit :=
+mcond tags_enabled
+  (do in_tag ← get_main_tag,
+      r ← tac,
+      /- remove assigned metavars -/
+      r ← r.mfilter $ λ ⟨n, m⟩, bnot <$> is_assigned m,
+      match r with
+      | [(_, m)] := set_tag m in_tag /- if there is only new subgoal, we just propagate `in_tag` -/
+      | _        := r.mmap' (λ ⟨n, m⟩, set_tag m (n::in_tag))
+      end)
+  (tac >> skip)
+
+private meta def revert_new_hyps (input_hyp_uids : name_set) : m unit :=
+do ctx ← local_context,
+   let to_revert := ctx.foldr (λ h r, if input_hyp_uids.contains h.local_uniq_name then r else h::r) [],
+   tag ← get_main_tag,
+   m   ← revert_lst to_revert,
+   set_main_tag (mk_num_name `_case m :: tag)
+end
+
+namespace interactive
+section
+open tactic.interactive
+parameters {m n : Type → Type} [monad_tactic m] [monad_state_lift tag_info n m] [monad n]
+include n
+
+private meta def collect_hyps_uids : m name_set :=
+do ctx ← local_context,
+   return $ ctx.foldl (λ r h, r.insert h.local_uniq_name) mk_name_set
+
+/--
+Apply `t` to main goal, and revert any new hypothesis in the generated goals,
+and tag generated goals when using supported tactics such as: `induction`, `apply`, `cases`, `constructor`, ...
+
+This tactic is useful for writing robust proof scripts that are not sensitive
+to the name generation strategy used by `t`.
+
+```
+example (n : ℕ) : n = n :=
+begin
+  with_cases { induction n },
+  case nat.zero { reflexivity },
+  case nat.succ : n' ih { reflexivity }
+end
+```
+
+TODO(Leo): improve docstring
+-/
+meta def with_cases (t : itactic) : m unit :=
+with_enable_tags $ focus1 $ do
+  input_hyp_uids ← collect_hyps_uids,
+  t,
+  all_goals (revert_new_hyps input_hyp_uids)
+
+/--
+  Given the initial tag `in_tag` and the cases names produced by `induction` or `cases` tactic,
+  update the tag of the new subgoals.
+-/
+private meta def set_cases_tags (in_tag : tag) (rs : list name) : m unit :=
+do te ← tags_enabled,
+   gs ← get_goals,
+   match gs with
+   | [g] := when te (set_tag g in_tag) -- if only one goal was produced, we should not make the tag longer
+   | _   := do
+     let tgs : list (name × expr) := rs.map₂ (λ n g, (n, g)) gs,
+     if te
+     then tgs.mmap' (λ ⟨n, g⟩, set_tag g (n::in_tag))
+          /- If `induction/cases` is not in a `with_cases` block, we still set tags using `_case_simple` to make
+             sure we can use the `case` notation.
+             ```
+             induction h,
+             case c { ... }
+             ```
+          -/
+     else tgs.mmap' (λ ⟨n, g⟩, with_enable_tags (set_tag g (`_case_simple::n::[])))
+   end
+
+private meta def set_induction_tags (in_tag : tag) (rs : list (name × list expr × list (name × expr))) : m unit :=
+set_cases_tags in_tag (rs.map (λ e, e.1))
+
+private meta def is_case_simple_tag : tag → bool
+| (`_case_simple :: _) := tt
+| _                    := ff
+
+private meta def is_case_tag : tag → option nat
+| (name.mk_numeral n `_case :: _) := some n.val
+| _                               := none
+
+private meta def tag_match (t : tag) (pre : list name) : bool :=
+pre.is_prefix_of t.reverse &&
+((is_case_tag t).is_some || is_case_simple_tag t)
+
+private meta def collect_tagged_goals (pre : list name) : m (list expr) :=
+do gs ← get_goals,
+   gs.mfoldr (λ g r, do
+      t ← get_tag g,
+      if tag_match t pre then return (g::r) else return r)
+      []
+
+private meta def find_tagged_goal_aux (pre : list name) : m expr :=
+do gs ← collect_tagged_goals pre,
+   match gs with
+   | []  := fail ("invalid `case`, there is no goal tagged with prefix " ++ to_string pre)
+   | [g] := return g
+   | gs  := do
+     tags : list (list name) ← gs.mmap get_tag,
+     monad_lift $ fail ("invalid `case`, there is more than one goal tagged with prefix " ++ to_string pre ++ ", matching tags: " ++ to_string tags)
+   end
+
+private meta def find_tagged_goal (pre : list name) : m expr :=
+match pre with
+| [] := do g::gs ← get_goals, return g
+| _  :=
+  find_tagged_goal_aux pre
+  <|>
+  -- try to resolve constructor names, and try again
+  do env ← get_env,
+     pre ← pre.mmap (λ id,
+           (do r_id ← resolve_constant id,
+               if (env.inductive_type_of r_id).is_none then return id
+               else return r_id)
+            <|> return id),
+     find_tagged_goal_aux pre
+end
+
+private meta def find_case (goals : list expr) (ty : name) (idx : nat) (num_indices : nat) : option expr → expr → option (expr × expr)
+| case e := if e.has_meta_var then match e with
+  | (mvar _ _ _)    :=
+    do case ← case,
+       guard $ e ∈ goals,
+       pure (case, e)
+  | (app _ _)    :=
+    let idx :=
+      match e.get_app_fn with
+      | const (name.mk_string rec ty') _ :=
+        guard (ty' = ty) >>
+        match mk_simple_name rec with
+        | `drec := some idx | `rec := some idx
+        -- indices + major premise
+        | `dcases_on := some (idx + num_indices + 1) | `cases_on := some (idx + num_indices + 1)
+        | _ := none
+        end
+      | _ := none
+      end in
+    match idx with
+    | none := list.foldl (<|>) (find_case case e.get_app_fn) $ e.get_app_args.map (find_case case)
+    | some idx :=
+      let args := e.get_app_args in
+      do arg ← args.nth idx,
+         args.enum.foldl
+           (λ acc ⟨i, arg⟩, match acc with
+             | some _ := acc
+             | _      := if i ≠ idx then find_case none arg else none
+             end)
+           -- start recursion with likely case
+           (find_case (some arg) arg)
+    end
+  | (lam _ _ _ e) := find_case case e
+  | (macro n args) := list.foldl (<|>) none $ args.map (find_case case)
+  | _             := none
+  end else none
+
+private meta def rename_lams : expr → list name → m unit
+| (lam n _ _ e) (n'::ns) := (rename n n' >> rename_lams e ns) <|> rename_lams e (n'::ns)
+| _             _        := skip
+
+/--
+Focuses on the `induction`/`cases`/`with_cases` subgoal corresponding to the given tag prefix, optionally renaming introduced locals.
+
+```
+example (n : ℕ) : n = n :=
+begin
+  induction n,
+  case nat.zero { reflexivity },
+  case nat.succ : a ih { reflexivity }
+end
+```
+-/
+meta def case (pre : parse ident_*) (ids : parse $ (tk ":" *> ident_*)?) (tac : itactic) : m unit :=
+do g   ← find_tagged_goal pre,
+   tag ← get_tag g,
+   let ids := ids.get_or_else [],
+   match is_case_tag tag with
+   | some n := do
+      let m := ids.length,
+      gs ← get_goals,
+      set_goals $ g :: gs.filter (≠ g),
+      intro_lst ids,
+      when (m < n) $ intron (n - m),
+      solve1 tac
+   | none   :=
+     match is_case_simple_tag tag with
+     | tt :=
+       /- Use the old `case` implementation -/
+       do r         ← result,
+          env       ← get_env,
+          [ctor_id] ← return pre,
+          ctor      ← resolve_constant ctor_id
+                      <|> fail ("'" ++ to_string ctor_id ++ "' is not a constructor"),
+          ty        ← (env.inductive_type_of ctor).to_monad
+                      <|> fail ("'" ++ to_string ctor ++ "' is not a constructor"),
+          let ctors := env.constructors_of ty,
+          let idx   := env.inductive_num_params ty + /- motive -/ 1 +
+                       list.index_of ctor ctors,
+          /- Remark: we now use `find_case` just to locate the `lambda` used in `rename_lams`.
+             The goal is now located using tags. -/
+          (case, _) ← (find_case [g] ty idx (env.inductive_num_indices ty) none r ).to_monad
+                      <|> fail "could not find open goal of given case",
+          gs        ← get_goals,
+          set_goals $ g :: gs.filter (≠ g),
+          rename_lams case ids,
+          solve1 tac
+     | ff := failed
+     end
+   end
+end ttactic
